wip

fstar/PPP.fst
@@ -269,10 +269,6 @@ let map_blocks_f_equiv_lemma
           assert (j < idx_start);
           proof_r2 j;
           assert (FStar.Seq.index r2 j == FStar.Seq.index updated_s j);
-          // FStar.Seq.lemma_index_slice updated_s 0 (i * blocksize) j;
-          // assert (FStar.Seq.index (FStar.Seq.slice updated_s 0 (i * blocksize)) j == FStar.Seq.index updated_s (j + 0));
-          // assert (FStar.Seq.index acc j == FStar.Seq.index original_s (j + 0));
-          // assert (FStar.Seq.index updated_s j == FStar.Seq.index original_s j);
           assert (FStar.Seq.index r1 j == FStar.Seq.index r2 j);
           ()
         )
@@ -280,78 +276,105 @@ let map_blocks_f_equiv_lemma
     FStar.Classical.forall_intro proof
 #pop-options
 
-
-
-// #push-options "--z3rlimit 100"
-// let map_blocks_f_equiv_lemma
-//   (len: uint_size) (blocksize: size_pos)
-//   (max: uint_size {max * blocksize <= len})
-//   (original_s: lseq 'a len)
-//   (f:(i:nat{i < max}) -> lseq 'a blocksize -> lseq 'a blocksize)
-//   (i: nat{i < max})
-//   (acc: lseq 'a (i * blocksize) {Seq.equal acc (FStar.Seq.slice s0 0 (i * blocksize))})
-//   : Lemma (
-//           let slice_s = FStar.Seq.slice s0 0 (max * blocksize) in
-//           forall (j: nat{j < (i+1) * blocksize}).
-//             FStar.Seq.index (Seq.map_blocks_f blocksize max slice_s f i acc) j
-//          == FStar.Seq.index (seq_set_exact_chunk #_ #len s0 blocksize i (f i (seq_get_exact_chunk s0 blocksize i))) j
-//     )
-//   = let slice_s = FStar.Seq.slice s0 0 (max * blocksize) in
-//     Math.Lemmas.lemma_mult_le_right blocksize (i+1) max;
-//     let block = FStar.Seq.slice s0 (i*blocksize) ((i+1)*blocksize) in
-//     let r1 = FStar.Seq.append acc (f i block) in
-//     assert (r1 == Seq.map_blocks_f blocksize max slice_s f i acc);
-
-//     let idx_start = blocksize * i in
-//     let out_len = seq_chunk_len s0 blocksize i in
-//     let new_block = f i (seq_get_exact_chunk s0 blocksize i) in
-//     let r2 = Seq.update_sub s0 idx_start out_len new_block in
-//     assert (seq_chunk_len s0 blocksize i == (
-//       if blocksize * (i + 1) > Seq.length s0
-//       then (if blocksize * i < Seq.length s0
-//             then sub_rem_lemma i (Seq.length s0) blocksize;
-//             Seq.length s0 % blocksize)
-//       else blocksize
-//     ));
-//     let proof_r2 (k:nat{(0 <= k /\ k < idx_start) \/ (idx_start + out_len <= k /\ k < len)}): Lemma (Seq.index r2 k == Seq.index s0 k) = () in
-//     assert (seq_set_exact_chunk #_ #len s0 blocksize i new_block == r2);
-//     let proof (j:nat{j < (i+1) * blocksize})
-//       : Lemma (FStar.Seq.index r1 j == FStar.Seq.index r2 j)
-//       = if j >= i * blocksize
-//         then (
-//           assert (FStar.Seq.index r1 j == FStar.Seq.index (f i block) (j - i * blocksize));
-//           assert (FStar.Seq.index r2 j == FStar.Seq.index (f i block) (j - i * blocksize));
-//           assert (FStar.Seq.index r1 j == FStar.Seq.index r2 j)
-//         ) else (
-//           assert (FStar.Seq.index r1 j == FStar.Seq.index acc j);
-//           assert (FStar.Seq.index r1 j == FStar.Seq.index s0 j);
-//           assert (i < max /\ max * blocksize <= len);
-//           assert ((i+1) * blocksize <= len ==> j < len);
-//           assert (j < len);
-//           assert (j < idx_start);
-//           proof_r2 j;
-//           assert (FStar.Seq.index r2 j == FStar.Seq.index s0 j);
-//           assert (FStar.Seq.index r1 j == FStar.Seq.index r2 j);
-//           ()
-//         )
-//     in
-//     FStar.Classical.forall_intro proof
-// #pop-options
-
-let map_blocks_foldi_fun
+unfold let map_blocks_foldi_fun
   (len: uint_size) (blocksize: size_pos)
   (max: uint_size {max * blocksize <= len})
   (f:(i:nat{i < max}) -> lseq 'a blocksize -> lseq 'a blocksize)
-  = fun i (s: lseq 'a len) -> seq_set_exact_chunk #_ #len s blocksize i (f i (seq_get_exact_chunk s blocksize i))
+  (i: nat{i<max}) (s: lseq 'a len)
+  = seq_set_exact_chunk #_ #len s blocksize i (f i (seq_get_exact_chunk s blocksize i))
 
-let map_blocks_foldi
-    (len: uint_size) (blocksize: size_pos)
+#push-options "--z3rlimit 40"
+let map_blocks_foldi_fun_preserve_above
+  (len: uint_size) (blocksize: size_pos)
+  (max: uint_size {max * blocksize <= len})
+  (f:(i:nat{i < max}) -> lseq 'a blocksize -> lseq 'a blocksize)
+  (i: nat{i < max}) (s: lseq 'a len)
+  : Lemma (
+    forall (j:nat{j >= blocksize * (i+1) /\ j < len}).
+       FStar.Seq.index (map_blocks_foldi_fun len blocksize max f i s) j
+    == FStar.Seq.index s j
+  )
+  = let r = seq_set_exact_chunk #_ #len s blocksize i (f i (seq_get_exact_chunk s blocksize i)) in
+    let idx_start = blocksize * i in
+    let out_len = seq_chunk_len s blocksize i in
+    assert (out_len == (
+      if blocksize * (i + 1) > Seq.length s
+      then (if blocksize * i < Seq.length s
+            then sub_rem_lemma i (Seq.length s) blocksize;
+            Seq.length s % blocksize)
+      else blocksize
+    ));
+    let r'
+        = Seq.update_sub s idx_start out_len (f i (seq_get_exact_chunk s blocksize i)) in
+    assert ((forall (k:nat{(0 <= k /\ k < blocksize * i) \/ (blocksize * i + out_len <= k /\ k < len)}).
+       Seq.index r' k == Seq.index s k));
+    if blocksize * (i + 1) > Seq.length s
+    then assert (false)
+    else introduce forall (j:nat{j >= blocksize * (i+1) /\ j < len}). Seq.index r' j == Seq.index s j
+              with ()
+
+unfold let map_blocks_foldi
+    (#len: uint_size) (blocksize: size_pos)
     (max: uint_size {max * blocksize <= len})
     (n: uint_size {n * blocksize <= len /\ n <= max})
     (s: lseq 'a len)
     (f:(i:nat{i < max}) -> lseq 'a blocksize -> lseq 'a blocksize)
     : lseq 'a len
   = foldi 0 n (map_blocks_foldi_fun len blocksize max f) s
+
+let rec foldi_extensionality_squash
+  (lo: uint_size)
+  (hi: uint_size{lo <= hi})
+  (f: (i:uint_size{i < hi}) -> 'a -> 'a)
+  (g: (i:uint_size{i < hi}) -> 'a -> 'a {forall i x. f i x == g i x})
+  (init: 'a)
+  : squash (foldi lo hi f init == foldi lo hi g init)
+  = if lo = hi
+    then ( unfold_foldi lo hi f init;
+           unfold_foldi lo hi g init
+         )
+    else ( unfold_left_foldi lo hi f init;
+           unfold_left_foldi lo hi g init;
+           foldi_extensionality_squash lo (hi - 1) f g init
+         )
+
+let foldi_extensionality
+  (lo: uint_size)
+  (hi: uint_size{lo <= hi})
+  (f: (i:uint_size{i < hi}) -> 'a -> 'a)
+  (g: (i:uint_size{i < hi}) -> 'a -> 'a {forall i x. f i x == g i x})
+  (init: 'a)
+  : Lemma (foldi lo hi f init == foldi lo hi g init)
+  = foldi_extensionality_squash lo hi f g init
+
+#push-options "--ifuel 0 --fuel 0 --z3rlimit 15 --split_queries"
+let map_blocks_foldi_fun_simplify
+  (#len: uint_size) (blocksize: size_pos)
+  (max: uint_size {max * blocksize <= len})
+  (n: uint_size {n * blocksize <= len /\ n <= max})
+  (s: lseq 'a len)
+  (f:(i:nat{i < max}) -> lseq 'a blocksize -> lseq 'a blocksize)
+  : squash (
+       foldi 0 n (map_blocks_foldi_fun len blocksize max f) s
+    == foldi 0 n (fun (i: nat{i<max}) (s: lseq 'a len) -> seq_set_exact_chunk #'a #len s blocksize i (f i (seq_get_exact_chunk s blocksize i))) s
+  ) = foldi_extensionality_squash 0 n
+                                  (map_blocks_foldi_fun len blocksize max f)
+                                  (fun (i: nat{i<max}) (s: lseq 'a len) -> seq_set_exact_chunk #'a #len s blocksize i (f i (seq_get_exact_chunk s blocksize i)))
+                                  s
+#pop-options
+
+#push-options "--z3rlimit 20 --split_queries"
+let map_blocks_foldi_simplify
+  (#len: uint_size) (blocksize: size_pos)
+  (max: uint_size {max * blocksize <= len})
+  (n: uint_size {n * blocksize <= len /\ n <= max})
+  (s: lseq 'a len)
+  (f:(i:nat{i < max}) -> lseq 'a blocksize -> lseq 'a blocksize)
+  : Lemma (
+       map_blocks_foldi blocksize max n s f
+    == foldi 0 n (fun (i: nat{i<max}) (s: lseq 'a len) -> seq_set_exact_chunk #'a #len s blocksize i (f i (seq_get_exact_chunk s blocksize i))) s
+  ) = map_blocks_foldi_fun_simplify blocksize max n s f
+#pop-options
 
 #push-options "--z3rlimit 40"
 let rec map_blocks_foldi_preserves
@@ -360,24 +383,27 @@ let rec map_blocks_foldi_preserves
     (n: uint_size {n * blocksize <= len /\ n <= max})
     (s0: lseq 'a len)
     (f:(i:nat{i < max}) -> lseq 'a blocksize -> lseq 'a blocksize)
-  : Lemma (
-      (forall (i:nat{i >= blocksize * n /\ i < len}). FStar.Seq.index s0 i == FStar.Seq.index (map_blocks_foldi len blocksize max n s0 f) i)
-    ) =
-      if n = 0
-      then unfold_foldi 0 n (map_blocks_foldi_fun len blocksize max f) s0
-      else (
-        unfold_left_foldi 0 n (map_blocks_foldi_fun len blocksize max f) s0;
-        assert (
-             map_blocks_foldi_fun len blocksize max f (n - 1) (map_blocks_foldi len blocksize max (n - 1) s0 f)
-          == map_blocks_foldi len blocksize max n s0 f
-        );
-        map_blocks_foldi_preserves len blocksize max (n - 1) s0 f;
-        admit ()
-      )
+  : Lemma (forall (i:nat{i >= blocksize * n /\ i < len}). FStar.Seq.index s0 i == FStar.Seq.index (map_blocks_foldi blocksize max n s0 f) i)
+   = if n = 0
+     then unfold_foldi 0 0 (map_blocks_foldi_fun len blocksize max f) s0
+     else (
+       unfold_left_foldi 0 n (map_blocks_foldi_fun len blocksize max f) s0;
+       assert (
+            map_blocks_foldi_fun len blocksize max f (n - 1) (map_blocks_foldi blocksize max (n - 1) s0 f)
+         == map_blocks_foldi blocksize max n s0 f
+       );
+       map_blocks_foldi_preserves len blocksize max (n - 1) s0 f;
+       assert (forall (i:nat{i >= blocksize * (n-1) /\ i < len}). FStar.Seq.index s0 i == FStar.Seq.index (map_blocks_foldi blocksize max (n-1) s0 f) i);
+       introduce forall (i: nat{i < max}) (s: lseq 'a len). forall (j:nat{j >= blocksize * (i+1) /\ j < len}).
+                          FStar.Seq.index (map_blocks_foldi_fun len blocksize max f i s) j
+                       == FStar.Seq.index s j
+            with map_blocks_foldi_fun_preserve_above len blocksize max f i s;
+       ()
+     )
 #pop-options
 
 #push-options "--print_implicits"
-let direct_statement
+unfold let direct_statement
     (len: uint_size) (blocksize: size_pos)
     (max: uint_size {max * blocksize <= len})
     (n: uint_size {n * blocksize <= len /\ n <= max})
@@ -385,8 +411,7 @@ let direct_statement
     (f:(i:nat{i < max}) -> lseq 'a blocksize -> lseq 'a blocksize)
   = let slice_s = FStar.Seq.slice s 0 (max * blocksize) in
     let r1: Seq.map_blocks_a 'a blocksize max n = LC.repeat_gen n (Seq.map_blocks_a 'a blocksize max) (Seq.map_blocks_f blocksize max slice_s f) FStar.Seq.empty in
-    // let r2 = foldi 0 n (fun i (s: lseq 'a len) -> seq_set_exact_chunk #_ #len s blocksize i (f i (seq_get_exact_chunk s blocksize i))) s in
-    let r2 = map_blocks_foldi len blocksize max n s f in
+    let r2 = map_blocks_foldi blocksize max n s f in
     (forall (i:nat{i < blocksize * n}). FStar.Seq.index r1 i == FStar.Seq.index r2 i)
 
 // #push-options "--fuel 0 --ifuel 0 --z3rlimit 150 --split_queries"
@@ -397,258 +422,27 @@ let rec direct
   (n: uint_size {n * blocksize <= len /\ n <= max})
   (s: lseq 'a len)
   (f:(i:nat{i < max}) -> lseq 'a blocksize -> lseq 'a blocksize)
-  : Lemma (ensures (
-      direct_statement len blocksize max n s f
-      // let slice_s = FStar.Seq.slice s 0 (max * blocksize) in
-      // let r1: Seq.map_blocks_a 'a blocksize max n = LC.repeat_gen n (Seq.map_blocks_a 'a blocksize max) (Seq.map_blocks_f blocksize max slice_s f) FStar.Seq.empty in
-      // true
-      // let r2 = foldi 0 n (fun i (s: lseq 'a len) -> seq_set_exact_chunk #_ #len s blocksize i (f i (seq_get_exact_chunk s blocksize i))) s in
-      // let r2 = map_blocks_foldi len blocksize max n s f in
-      // forall (i:nat{i < blocksize * n}). FStar.Seq.index r1 i == FStar.Seq.index r2 i
-    )) (decreases n)
-  = if n = 0
-    then ()
-    else begin
+  : Lemma (ensures direct_statement len blocksize max n s f) (decreases n)
+  = if n <> 0 then begin
       let n': uint_size = n - 1 in
       let slice_s = FStar.Seq.slice s 0 (max * blocksize) in
       
-      let r1': s:seq 'a{Seq.length s == (n - 1) * blocksize} = LC.repeat_gen (n-1) (Seq.map_blocks_a 'a blocksize max) (Seq.map_blocks_f blocksize max slice_s f) FStar.Seq.empty in
-      // let r2' = foldi 0 (n-1) (fun i (s: lseq 'a len) -> seq_set_exact_chunk #_ #len s blocksize i (f i (seq_get_exact_chunk s blocksize i))) s in
-      let r2' = map_blocks_foldi len blocksize max (n - 1) s f in
+      let r1' = LC.repeat_gen (n-1) (Seq.map_blocks_a 'a blocksize max) (Seq.map_blocks_f blocksize max slice_s f) FStar.Seq.empty in
+      let r2' = map_blocks_foldi blocksize max (n - 1) s f in
       let all1 = Seq.map_blocks_f blocksize max slice_s f (n-1) r1' in
       let all2 = seq_set_exact_chunk #_ #len r2' blocksize (n-1) (f (n-1) (seq_get_exact_chunk r2' blocksize (n-1))) in
-      // let _ =
-        let _: squash (forall (i:nat{i < blocksize * (n - 1)}). FStar.Seq.index r1' i == FStar.Seq.index r2' i)
-          = assert_norm (direct_statement len blocksize max (n - 1) s f == (forall (i:nat{i < blocksize * (n - 1)}). FStar.Seq.index r1' i == FStar.Seq.index r2' i));
-            direct len blocksize max (n - 1) s f
-        in
-        map_blocks_foldi_preserves len blocksize max (n-1) s f;
-        map_blocks_f_equiv_lemma len blocksize max s f (n-1) r2' r1';
-        assert (forall (j: nat{j < n * blocksize}). FStar.Seq.index all1 j == FStar.Seq.index all2 j);
-      unfold_left_foldi 0 n (map_blocks_foldi_fun len blocksize max f) s;
-      // unfold_left_foldi 0 n (fun i (s: lseq 'a len) -> seq_set_exact_chunk #_ #len s blocksize i (f i (seq_get_exact_chunk s blocksize i))) s;
-      LC.unfold_repeat_gen n (Seq.map_blocks_a 'a blocksize max) (Seq.map_blocks_f blocksize max slice_s f) FStar.Seq.empty (n - 1);
-        ()
-    end
-#pop-options
-
-
-
-
-
-
-
-
-
-
-
-
-
-
-
-
-
-
-
-
-let direct_statement
-    (len: uint_size) (blocksize: size_pos)
-    (max: uint_size {max * blocksize <= len})
-    (n: uint_size {n * blocksize <= len /\ n <= max})
-    (s: lseq 'a len)
-    (f:(i:nat{i < max}) -> lseq 'a blocksize -> lseq 'a blocksize)
-  = let slice_s = FStar.Seq.slice s 0 (max * blocksize) in
-    let r1: Seq.map_blocks_a 'a blocksize max n = LC.repeat_gen n (Seq.map_blocks_a 'a blocksize max) (Seq.map_blocks_f blocksize max slice_s f) FStar.Seq.empty in
-    let r2 = foldi 0 n (fun i (s: lseq 'a len) -> seq_set_exact_chunk #_ #len s blocksize i (f i (seq_get_exact_chunk s blocksize i))) s in
-    (forall (i:nat{i < blocksize * n}). FStar.Seq.index r1 i == FStar.Seq.index r2 i)
-
-#push-options "--fuel 0 --ifuel 0 --z3rlimit 150 --split_queries"
-let rec direct
-  (len: uint_size) (blocksize: size_pos)
-  (max: uint_size {max * blocksize <= len})
-  (n: uint_size {n * blocksize <= len /\ n <= max})
-  (s: lseq 'a len)
-  (f:(i:nat{i < max}) -> lseq 'a blocksize -> lseq 'a blocksize)
-  : Lemma (ensures (
-      direct_statement len blocksize max n s f
-      // let slice_s = FStar.Seq.slice s 0 (max * blocksize) in
-      // let r1: Seq.map_blocks_a 'a blocksize max n = LC.repeat_gen n (Seq.map_blocks_a 'a blocksize max) (Seq.map_blocks_f blocksize max slice_s f) FStar.Seq.empty in
-      // true
-      // let r2 = foldi 0 n (fun i (s: lseq 'a len) -> seq_set_exact_chunk #_ #len s blocksize i (f i (seq_get_exact_chunk s blocksize i))) s in
-      // let r2 = map_blocks_foldi len blocksize max n s f in
-      // forall (i:nat{i < blocksize * n}). FStar.Seq.index r1 i == FStar.Seq.index r2 i
-    )) (decreases n)
-  = if n = 0
-    then ()
-    else begin
-      let n': uint_size = n - 1 in
-      let slice_s = FStar.Seq.slice s 0 (max * blocksize) in
-      // unfold_left_foldi 0 n (fun i (s: lseq 'a len) -> seq_set_exact_chunk #_ #len s blocksize i (f i (seq_get_exact_chunk s blocksize i))) s;
-      // LC.unfold_repeat_gen n (Seq.map_blocks_a 'a blocksize max) (Seq.map_blocks_f blocksize max slice_s f) FStar.Seq.empty (n - 1);
-      
-      let r1': s:seq 'a{Seq.length s == (n - 1) * blocksize} = LC.repeat_gen (n-1) (Seq.map_blocks_a 'a blocksize max) (Seq.map_blocks_f blocksize max slice_s f) FStar.Seq.empty in
-      let r2' = foldi 0 (n-1) (fun i (s: lseq 'a len) -> seq_set_exact_chunk #_ #len s blocksize i (f i (seq_get_exact_chunk s blocksize i))) s in
-      let all1 = Seq.map_blocks_f blocksize max slice_s f (n-1) r1' in
-      let all2 = seq_set_exact_chunk #_ #len r2' blocksize (n-1) (f (n-1) (seq_get_exact_chunk r2' blocksize (n-1))) in
-      let _ =
-        let _: squash (forall (i:nat{i < blocksize * (n - 1)}). FStar.Seq.index r1' i == FStar.Seq.index r2' i)
-          = assert_norm (direct_statement len blocksize max (n - 1) s f == (forall (i:nat{i < blocksize * (n - 1)}). FStar.Seq.index r1' i == FStar.Seq.index r2' i));
-            direct len blocksize max (n - 1) s f
-        in
-        map_blocks_foldi_preserves len blocksize max (n-1) s f;
-        map_blocks_f_equiv_lemma len blocksize max s f (n-1) r2' r1';
-        assert (
-          let slice_s = FStar.Seq.slice s 0 (max * blocksize) in
-            forall (j: nat{j < n * blocksize}).
-             FStar.Seq.index all1 j
-          == FStar.Seq.index all2 j
-        );
-        ()
+      let _: squash (forall (i:nat{i < blocksize * (n - 1)}). FStar.Seq.index r1' i == FStar.Seq.index r2' i)
+        = direct len blocksize max (n - 1) s f;
+          assert (direct_statement len blocksize max (n - 1) s f);
+          assert ((forall (i:nat{i < blocksize * (n - 1)}). FStar.Seq.index r1' i == FStar.Seq.index r2' i))
       in
-      // admitP ( Seq.map_blocks_f blocksize max slice_s f (n - 1) r1'
-      //       == seq_set_exact_chunk #_ #len s blocksize (n - 1) (f (n - 1) (seq_get_exact_chunk s blocksize (n - 1)))
-      // );
-      admit ()
+      map_blocks_foldi_preserves len blocksize max (n-1) s f;
+      map_blocks_f_equiv_lemma len blocksize max s f (n-1) r2' r1';
+      assert (forall (j: nat{j < n * blocksize}). FStar.Seq.index all1 j == FStar.Seq.index all2 j);
+      unfold_left_foldi 0 n (map_blocks_foldi_fun len blocksize max f) s;
+      LC.unfold_repeat_gen n (Seq.map_blocks_a 'a blocksize max) (Seq.map_blocks_f blocksize max slice_s f) FStar.Seq.empty (n - 1)
     end
 #pop-options
-
-//   (len: uint_size)
-//   (blocksize: size_pos)
-//   (i: nat {i < blocksize / len})
-//   (inp: lseq 'a len)
-//   (f:(i:nat{i < max} -> lseq 'a blocksize -> lseq 'a blocksize))
-//   : Lemma (ensures (
-//     forall (i: nat {i < len})
-//     // Math.Lemmas.cancel_mul_div n blocksize;
-//     // // assert (n <= max ==> Lib.Sequence.length inp == max * blocksize ==> range (n * blocksize) U32);
-//     // admitP (range (n * blocksize) U32);
-//     // map_blocks_pointwise_spec (n * blocksize) blocksize
-//     //                           (fun i ->
-//     //                             f i (seq_get_exact_chunk inp blocksize i)
-//     //                           )
-//     //                           FStar.Seq.empty
-//     //                           (LC.repeat_gen n (Seq.map_blocks_a 'a blocksize max) (Seq.map_blocks_f blocksize max inp f) FStar.Seq.empty)
-//   ))
-
-
-
-
-
-
-
-
-
-
-
-
-
-
-
-#push-options "--z3rlimit 200"
-let map_blocks_multi_repeat_gen_lemma_pointwise_spec
-  (blocksize:size_pos)
-  (max: nat)
-  (n: nat {n <= max})
-  (inp: seq 'a {Lib.Sequence.length inp == max * blocksize})
-  (f:(i:nat{i < max} -> lseq 'a blocksize -> lseq 'a blocksize))
-  : Lemma (ensures (
-    Math.Lemmas.cancel_mul_div n blocksize;
-    // assert (n <= max ==> Lib.Sequence.length inp == max * blocksize ==> range (n * blocksize) U32);
-    admitP (range (n * blocksize) U32);
-    map_blocks_pointwise_spec (n * blocksize) blocksize
-                              (fun i ->
-                                f i (seq_get_exact_chunk inp blocksize i)
-                              )
-                              FStar.Seq.empty
-                              (LC.repeat_gen n (Seq.map_blocks_a 'a blocksize max) (Seq.map_blocks_f blocksize max inp f) FStar.Seq.empty)
-  ))
-  = let r = LC.repeat_gen n (Seq.map_blocks_a 'a blocksize max) (Seq.map_blocks_f blocksize max inp f) FStar.Seq.empty in
-    if n = 0
-    then
-      admit ()
-      // map_blocks_pointwise_spec'0 0 blocksize
-      //                         (fun i ->
-      //                           f i (seq_get_exact_chunk inp blocksize i)
-      //                         )
-      //                         FStar.Seq.empty
-      //                         (LC.repeat_gen n (Seq.map_blocks_a 'a blocksize max) (Seq.map_blocks_f blocksize max inp f) FStar.Seq.empty)
-    else (
-      let n': nat = n - 1 in
-      LC.unfold_repeat_gen max (Seq.map_blocks_a 'a blocksize max) (Seq.map_blocks_f blocksize max inp f) FStar.Seq.empty n';
-      let acc = LC.repeat_gen n' (Seq.map_blocks_a 'a blocksize max) (Seq.map_blocks_f blocksize max inp f) FStar.Seq.empty in
-      Math.Lemmas.lemma_mult_le_right blocksize (n'+1) max;
-      let block = FStar.Seq.slice inp (n'*blocksize) ((n'+1)*blocksize) in
-      let result = FStar.Seq.append acc (f n' block) in
-      introduce forall k. FStar.Seq.index (FStar.Seq.slice inp (n'*blocksize) ((n'+1)*blocksize)) k == FStar.Seq.index inp (k + (n'*blocksize))
-           with FStar.Seq.lemma_index_slice inp (n'*blocksize) ((n'+1)*blocksize) k;
-      introduce forall (i:nat{i < (n'+1)*blocksize}). FStar.Seq.index result i == (if i < n' * blocksize
-                                                                            then FStar.Seq.index acc i
-                                                                            else FStar.Seq.index (f n' block) (i - n' * blocksize)
-                                                                            )
-           with begin
-                  if i < n' * blocksize 
-                  then FStar.Seq.lemma_index_app1 acc (f n' block) i
-                  else FStar.Seq.lemma_index_app2 acc (f n' block) i
-                end;
-      assert (r == result);
-      ()
-    )
-#pop-options
-
-#push-options "--z3rlimit 50"
-let map_blocks_multi_lemma_pointwise_spec
-  (blocksize:size_pos)
-  (max: nat)
-  (n: nat {n <= max})
-  (inp: seq 'a {Lib.Sequence.length inp == max * blocksize})
-  (f:(i:nat{i < max} -> lseq 'a blocksize -> lseq 'a blocksize))
-  : Lemma (ensures (
-    Math.Lemmas.cancel_mul_div n blocksize;
-    map_blocks_pointwise_spec (n * blocksize) blocksize
-                              (fun i ->
-                                f i (seq_get_exact_chunk inp blocksize i)
-                              )
-                              FStar.Seq.empty
-                              (Seq.map_blocks_multi blocksize max n inp f)
-  ))
-  = Seq.lemma_map_blocks_multi blocksize max n inp f;
-    let r' = Seq.map_blocks_multi blocksize max n inp f in
-    let r = LC.repeat_gen n (Seq.map_blocks_a 'a blocksize max) (Seq.map_blocks_f blocksize max inp f) FStar.Seq.empty in
-    map_blocks_multi_repeat_gen_lemma_pointwise_spec blocksize max n inp f
-#pop-options
-
-
-#push-options "--z3rlimit 500 --split_queries"
-let map_blocks_lemma_pointwise_spec
-  (#len: uint_size)
-  (blocksize:size_pos)
-  (inp:lseq 'a len)
-  (f:(Seq.block len blocksize -> lseq 'a blocksize -> lseq 'a blocksize))
-  (g:(Seq.last len blocksize -> rem:size_nat{rem < blocksize} -> s:lseq 'a rem -> lseq 'a rem))
-  : Lemma (
-    // true
-    map_blocks_pointwise_spec len blocksize
-                              (fun i -> f i (seq_get_exact_chunk inp blocksize i))
-                              (g (len / blocksize)
-                                 (len % blocksize)
-                                 (seq_get_remainder_chunk_length_lemma inp blocksize;
-                                  seq_get_remainder_chunk inp blocksize)
-                              )
-                              (Seq.map_blocks blocksize inp f g)
-  )
-  = Seq.lemma_map_blocks blocksize inp f g;
-    let len = Lib.Sequence.length inp in
-    let nb = len / blocksize in
-    let rem = len % blocksize in
-    let blocks = FStar.Seq.slice inp 0 (nb * blocksize) in
-    let last = FStar.Seq.slice inp (nb * blocksize) len in
-    Math.Lemmas.cancel_mul_div nb blocksize;
-    let bs = Lib.Sequence.map_blocks_multi #'a blocksize nb nb blocks f in
-    let res = if (rem > 0) then FStar.Seq.append bs (g nb rem last) else bs in
-    assert (res == Seq.map_blocks #'a blocksize inp f g);
-    ()
-  #pop-options
-
 
 #push-options "--z3rlimit 160"
 let s_chacha20_update' (ctx: S.state) (cipher: seq (int_t U8 SEC)): (r:seq _{r==s_chacha20_update ctx cipher}) =
@@ -679,15 +473,97 @@ let s_chacha20_update' (ctx: S.state) (cipher: seq (int_t U8 SEC)): (r:seq _{r==
 #pop-options
 
 
+// let map_blocks_foldi_simplify
+//   (#len: uint_size) (blocksize: size_pos)
+//   (max: uint_size {max * blocksize <= len})
+//   (n: uint_size {n * blocksize <= len /\ n <= max})
+//   (s: lseq 'a len)
+//   (f:(i:nat{i < max}) -> lseq 'a blocksize -> lseq 'a blocksize)
+//   : Lemma (
+//        map_blocks_foldi blocksize max n s f
+//     == foldi 0 n (fun (i: nat{i<max}) (s: lseq 'a len) -> seq_set_exact_chunk #'a #len s blocksize i (f i (seq_get_exact_chunk s blocksize i))) s
+//   ) = map_blocks_foldi_fun_simplify blocksize max n s f
 
-let chacha20_update_ (st0 : state_t) (cipher : byte_seq) : r:byte_seq{r == chacha20_update st0 cipher} =
+
+let chacha20_update0 (st0 : state_t) (cipher : byte_seq): lseq uint8 (FStar.Seq.length cipher) =
   let blocks_out: seq uint8 = seq_new_ (secret (pub_u8 0x0)) (seq_len cipher) in
   let n_blocks: uint_size = seq_num_exact_chunks cipher 64 in
+  
   let f (i: nat {i<n_blocks}): block_t = 
     let msg_block: seq uint8 = seq_get_exact_chunk cipher 64 i in
     chacha20_encrypt_block st0 (secret (pub_u32 i)) (array_from_seq 64 msg_block)
   in
-  let blocks_out = IC.map_blocks_foldi'0 64 0 n_blocks f blocks_out in
+  foldi 0 n_blocks (fun (i: uint_size{i<n_blocks}) (s: lseq _ (seq_len #uint8 cipher)) -> seq_set_exact_chunk s 64 i (f i)) blocks_out
+
+let chacha20_update0' (st0 : state_t) (cipher : byte_seq): lseq uint8 (FStar.Seq.length cipher) =
+  let blocks_out: seq uint8 = seq_new_ (secret (pub_u8 0x0)) (seq_len cipher) in
+  let n_blocks: uint_size = seq_num_exact_chunks cipher 64 in
+
+    
+  let f0 (i: nat {i<n_blocks}): block_t = 
+    let msg_block: seq uint8 = seq_get_exact_chunk cipher 64 i in
+    chacha20_encrypt_block st0 (secret (pub_u32 i)) (array_from_seq 64 msg_block)
+  in
+  let r0 = foldi 0 n_blocks (fun (i: uint_size{i<n_blocks}) (s: lseq uint8 (seq_len #uint8 cipher)) -> seq_set_exact_chunk #uint8 #(seq_len #uint8 cipher) s 64 i (f0 i)) blocks_out in
+  
+  // let r1 = foldi 0 n_blocks (fun (i: uint_size{i<n_blocks}) (s: lseq uint8 (FStar.Seq.length #uint8 cipher)) -> seq_set_exact_chunk s 64 i (f0 i)) blocks_out in
+  // let proof
+  //   : squash (
+  //      foldi 0 n_blocks (fun (i: uint_size{i<n_blocks}) (s: lseq uint8 (seq_len #uint8 cipher)) -> seq_set_exact_chunk #uint8 #(seq_len #uint8 cipher) s 64 i (f0 i)) blocks_out
+  //   == foldi 0 n_blocks (fun (i: uint_size{i<n_blocks}) (s: lseq uint8 (FStar.Seq.length #uint8 cipher)) -> seq_set_exact_chunk s 64 i (f0 i)) blocks_out
+  // ) =
+  //   foldi_extensionality 0 n_blocks (fun (i: uint_size{i<n_blocks}) (s: lseq uint8 (seq_len #uint8 cipher)) -> seq_set_exact_chunk #uint8 #(seq_len #uint8 cipher) s 64 i (f0 i))
+  //                                 (fun (i: uint_size{i<n_blocks}) (s: lseq uint8 (FStar.Seq.length #uint8 cipher)) -> seq_set_exact_chunk s 64 i (f0 i))
+  //                                 blocks_out in
+// assert (foldi 0 n_blocks (fun (i: uint_size{i<n_blocks}) (s: lseq uint8 (seq_len #uint8 cipher)) -> seq_set_exact_chunk #uint8 #(seq_len #uint8 cipher) s 64 i (f0 i)) blocks_out
+//     == foldi 0 n_blocks (fun (i: uint_size{i<n_blocks}) (s: lseq uint8 (FStar.Seq.length #uint8 cipher)) -> seq_set_exact_chunk s 64 i (f0 i)) blocks_out);
+//   assert (r0 == foldi 0 n_blocks (fun (i: uint_size{i<n_blocks}) (s: lseq uint8 (seq_len #uint8 cipher)) -> seq_set_exact_chunk #uint8 #(seq_len #uint8 cipher) s 64 i (f0 i)) blocks_out);
+//   assert (r1 == foldi 0 n_blocks (fun (i: uint_size{i<n_blocks}) (s: lseq uint8 (FStar.Seq.length #uint8 cipher)) -> seq_set_exact_chunk s 64 i (f0 i)) blocks_out);
+
+  let f2 (i: nat {i<n_blocks}) (msg_block: lseq uint8 64): block_t = 
+    chacha20_encrypt_block st0 (secret (pub_u32 i)) (array_from_seq 64 msg_block)
+  in
+  let r2 = map_blocks_foldi #uint8 #(seq_len cipher) 64 n_blocks n_blocks blocks_out f2 in
+
+  assert (r2 == r0) by (
+    norm [delta_only [`%map_blocks_foldi;`%map_blocks_foldi_fun;`%uint8]];
+    // compute ()
+    fail "x"
+  );
+
+  r0
+
+// let chacha20_update0_equiv (st0 : state_t) (cipher : byte_seq)
+//   : Lemma (chacha20_update0 st0 cipher == chacha20_update0' st0 cipher)
+//   = assert (chacha20_update0 st0 cipher == chacha20_update0' st0 cipher) by
+
+#push-options "--z3rlimit 160"
+let chacha20_update_ (st0 : state_t) (cipher : byte_seq) 
+  : r:byte_seq{r == chacha20_update st0 cipher} =
+  let blocks_out: seq uint8 = seq_new_ (secret (pub_u8 0x0)) (seq_len cipher) in
+  let n_blocks: uint_size = seq_num_exact_chunks cipher 64 in
+  
+  let f (i: nat {i<n_blocks}): block_t = 
+    let msg_block: seq uint8 = seq_get_exact_chunk cipher 64 i in
+    chacha20_encrypt_block st0 (secret (pub_u32 i)) (array_from_seq 64 msg_block)
+  in
+  let blocks_out = foldi 0 n_blocks (fun (i: uint_size{i<n_blocks}) (s: lseq uint8 (seq_len #uint8 cipher)) -> seq_set_exact_chunk #uint8 #(seq_len #uint8 cipher) s 64 i (f i)) blocks_out in
+  // let blocks_out' = foldi 0 n_blocks (fun (i: uint_size{i<n_blocks}) (s: lseq _ (Seq.length cipher)) -> seq_set_exact_chunk s 64 i (f i)) blocks_out in
+  
+  let last_block: seq uint8 = seq_get_remainder_chunk cipher 64 in
+  if seq_len last_block <> 0 then
+    let b : seq uint8 = chacha20_encrypt_last st0 (secret (pub_u32 n_blocks)) last_block in
+    seq_set_chunk (blocks_out <: lseq _ (seq_len cipher)) 64 n_blocks b
+  else blocks_out
+
+let chacha20_update_ (st0 : state_t) (cipher : byte_seq) =
+  // : byte_seq =
+  let blocks_out: seq uint8 = seq_new_ (secret (pub_u8 0x0)) (seq_len cipher) in
+  let n_blocks: uint_size = seq_num_exact_chunks cipher 64 in
+  let f (i: nat {i<n_blocks}) (msg_block: lseq uint8 64): block_t = 
+    chacha20_encrypt_block st0 (secret (pub_u32 i)) (array_from_seq 64 msg_block)
+  in
+  let blocks_out = map_blocks_foldi 64 n_blocks n_blocks blocks_out f in
   let last_block: seq uint8 = seq_get_remainder_chunk cipher 64 in
   if seq_len last_block <> 0 then
     let b : seq uint8 = chacha20_encrypt_last st0 (secret (pub_u32 n_blocks)) last_block in
